Added a proper kinding relation. Almost done with lifting and substitution lemmas.

src/Repr/SystemFOp/Type.v
@@ -81,6 +81,188 @@ Fixpoint typ_substitute (X:tvar)(U T:typ) : typ :=
 
 Notation "'[' X '|=>' U ']' T" := (typ_substitute X U T) (at level 30).
 
+(********************************************************************)
+(* We must define a Kind Judgement for Types *)
+
+Reserved Notation "D '\\-' T \: K" (at level 30).
+
+Inductive kind_rel : kenv -> typ -> kind -> Prop :=
+  | KR_TVar :
+      forall D X K,
+        get D X = Some K ->
+        D \\- TVar X \: K
+  | KR_TNat :
+      forall D,
+        D \\- TNat \: KStar
+  | KR_TArrow :
+      forall D T1 T2,
+        D \\- T1 \: KStar ->
+        D \\- T2 \: KStar ->
+        D \\- TArrow T1 T2 \: KStar
+  | KR_TAll :
+      forall D T,
+        (KStar :: D) \\- T \: KStar ->
+        D \\- TAll T \: KStar 
+
+where "D '\\-' T \: K" := (kind_rel D T K).
+
+Hint Constructors kind_rel.
+
+(* A couple of useful Lemma's --- I am cheating though, I saw these
+   from Iron Lambda *)
+
+(* Simple tactic that helps burn down the easy cases. *)
+Ltac inverts_typ :=
+  repeat
+    (match goal with
+       | [ H: _ \\- (TVar _)     \: _ |- _ ] => inverts H
+       | [ H: _ \\- TNat         \: _ |- _ ] => inverts H
+       | [ H: _ \\- (TArrow _ _) \: _ |- _ ] => inverts H
+       | [ H: _ \\- (TAll _)     \: _ |- _ ] => inverts H
+     end).
+
+(* This tactic 'usually' gets most of the inductive and easy cases
+ * when we induct over the typing relation. *)
+Tactic Notation "induction_kind" ident(t) :=
+  induction t; rip; simpl; inverts_typ; tburn.
+
+(* A well-kinded type is well-formed *)
+Lemma kind_rel_imp_well_formed_typ
+  :  forall D T K
+  ,  D \\- T \: K
+  -> well_formed_typ D T.
+Proof.
+  rip; gen D K; induction_kind T.
+Qed.
+
+(* We may insert into a kind environment at X provided we lift all
+ * types that occuring after X in the kind environment. 
+ *
+ * NOTE: This attempt at automation shows where the burn tactic fails,
+ * and one area where crush does well. Specifically, burn doesn't do
+ * a great job with rewriting after constructors are needed.
+ *
+ * It is tricky --- If you rewrite too soon or too late you will block
+ * the resolution process. Something I want to return to and study. *)
+Lemma kind_rel_insert
+  :  forall D T K X
+  ,  D \\- T \: K
+  -> insert D X KStar \\- typ_lift X T \: K.
+Proof.
+  Hint Rewrite insert_rewind.
+  rip; gen D K X; induction_kind T;
+  match goal with
+    (* TVar *)
+    | [ |- context [le_gt_dec ?A ?B] ] 
+      => break (le_gt_dec A B); tburn
+    (* TAbs *)
+    | _ 
+      => econstructor; autorewrite_goal; burn
+  end.
+  Remove Hints insert_rewind.
+Qed.
+Hint Resolve kind_rel_insert.
+
+Lemma cons_eq_insert0
+  :  forall X (ls: list X)(e:X)
+  ,  e :: ls = insert ls 0 e.
+Proof.
+  destruct ls; burn.
+Qed.  
+
+Theorem kind_rel_weakening
+  :  forall D T K
+  ,  D \\- T \: K
+  -> (KStar :: D) \\- typ_lift 0 T \: K.
+Proof.
+  rip; rewrite cons_eq_insert0; burn.
+Qed.  
+
+(********************************************************************)
+(* Lemmas for manipulating the lifting and substitution operations. *)
+
+(* Handy tactic for burning down TVar case analysis which usually boils down
+ * to repeated less than and nat compares *)
+Ltac burn_tvar :=
+  repeat(
+    simpl;
+    try break_nat_compare;
+    tburn;
+    match goal with
+      | [ |- context[le_gt_dec ?X ?Y] ] => break (le_gt_dec X Y)
+    end;
+    tburn
+  ).
+
+Ltac case_lift :=
+  match goal with
+    | [ |- context [le_gt_dec ?a ?b] ] =>
+      case (le_gt_dec a b)
+  end.
+
+Lemma typ_subs_nil_typ_lift
+  :  forall X U T
+  ,  [X |=> U] (typ_lift X T) = T.
+Proof.
+  rip; gen X U; induction_kind T; destruct X;
+  case_lift; burn_tvar. 
+Qed.
+Hint Rewrite typ_subs_nil_typ_lift.
+
+Lemma tall_injective 
+  :  forall (T1 T2:typ)
+  ,  T1 = T2
+  -> TAll T1 = TAll T2.
+Proof. burn. Qed.
+
+Lemma typ_lift_SX
+  :  forall (X Y:tvar)(T:typ)
+  ,  Y <= X
+  -> typ_lift Y (typ_lift X T) = typ_lift (S X) (typ_lift Y T).
+Proof.
+  rip; gen X Y; induction T; tburn.
+
+  rip;
+  rename t into Z;
+  break Z;
+  repeat(
+    simpl;
+    match goal with 
+      | [ |- context[le_gt_dec ?X ?Y] ] =>
+        break (le_gt_dec X Y)
+    end;
+    tburn
+  ).
+Qed.  
+
+Lemma typ_lift_over_subs
+  :  forall (n n':nat)(U T:typ)
+  ,  typ_lift n ([(n + n') |=> U] T) 
+  =  [(1 + n + n') |=> typ_lift n U] typ_lift n T.
+Proof.
+  rip; gen n n' U; induction T; tburn.
+  rip; burn_tvar.
+
+  rip; simpl; eapply tall_injective.
+  assert (S (n + n') = S n + n'). burn. rewrite H. rewrite IHT. simpl.
+  
+
+  rewrite <- typ_lift_SX; burn. 
+Qed.
+Hint Rewrite typ_lift_over_subs.
+
+(* LAST *)
+
+Lemma typ_lift_over_subs'
+  :  forall (n n':nat)(U T:typ)
+  ,  typ_lift (n + n') ([n |=> U] T) 
+  =  [n  |=> typ_lift (n + n') U] typ_lift (1 + n + n') T.
+Proof.
+  rip; gen n n' U; induction T; tburn.
+
+
+Qed.
+Hint Rewrite typ_lift_over_subs.
 
 (********************************************************************)
 
@@ -97,7 +279,6 @@ Hint Unfold tenv_lift.
 Definition tenv_substitute (X:tvar)(U:typ)(G:tenv) : tenv := 
   map (typ_substitute X U) G.
 Hint Unfold tenv_substitute.
-
 
 
 
